finish refactoring

definitions.v
@@ -18,22 +18,26 @@ Section Histories.
   Inductive invocation : Type :=
     | Inv : nat -> invocation.
   Inductive response : Type :=
-    | Resp : nat -> response.
+  | Resp : nat -> response
+  | NoResp.
   Definition invocation_eq (a1 a2: invocation) :=
     match a1, a2 with | Inv n, Inv n' => (n =? n') end.
   Definition response_eq (a1 a2: response) :=
-    match a1, a2 with | Resp n, Resp n' => (n =? n') end.
-
+    match a1, a2 with | Resp n, Resp n' => (n =? n')
+                   | NoResp, NoResp => true
+                   | _, _ => false
+    end.
   Inductive mode : Type :=
   | Commute : mode
   | Emulate : mode
   | Replay : mode.
 
   Definition action : Type := tid * invocation * response.
-  Definition action_eq a1 a2 :=
-    match a1, a2 with | (t1, Inv i1, Resp r1), (t2, Inv i2, Resp r2) =>
-                       (t1 =? t2) && (i1 =? i2) && (r1 =? r2) end.
-  Definition thread_of_action (a : action) := let '(t, Inv i1, Resp r1) := a in t.
+  Definition action_invocation_eq (a : action) (i : invocation) :=
+    match a, i with
+      | (_, Inv i1, _), Inv i2 => i1 =? i2
+    end.
+  Definition thread_of_action (a : action) := let '(t, _, _) := a in t.
                       
   Definition history : Type := list action.
   Definition base_history_pos_state : Type := tid -> nat.
@@ -45,13 +49,12 @@ Section Histories.
   Definition get_state_components s :=
     match s with | State bh ch md => (bh, ch, md) end.
 
-  Inductive event : Type := | NoEvent | Event (t: tid) (s1 s2 : state)
-                                              (i : invocation) (r : response) : event.
+  Inductive event : Type := | NoEvent | Event (s1 s2 : state) (a : action) : event.
   Definition trace : Type := list event.
   Function history_of_trace (tr: trace) : history :=
     match tr with
       | [] => []
-      | Event t s1 s2 a r :: tl => (t, a, r) :: history_of_trace tl
+      | Event s1 s2 a :: tl => a :: history_of_trace tl
       | _ :: tl => history_of_trace tl
     end.
   Function history_of_thread (h : history) (t : tid) : history :=
@@ -62,13 +65,13 @@ Section Histories.
     end.
   Definition trace_end_state (tr:trace) : option state :=
     match last tr NoEvent with
-      | Event t s1 s2 a r => Some s2
+      | Event s1 s2 a => Some s2
       | _ => None
     end.
     
   Definition swappable (a1 a2 : action) :=
     match a1, a2 with
-      | (t, Inv _, Resp _), (t', Inv _, Resp _) => t <> t'
+      | (t, _, _), (t',_, _) => t <> t'
     end.
   Inductive reordered : relation history :=
   | ro_perm_nil : reordered [] []
@@ -96,15 +99,14 @@ Section Commutativity.
     end.
  Function trace_writes (tr : trace) : Ensemble tid :=
     match tr with
-      | Event t s1 s2 a r :: tl =>
-        Union tid (step_writes s1 s2) (trace_writes tl)
+      | Event s1 s2 a :: tl => Union tid (step_writes s1 s2) (trace_writes tl)
       | _ => Empty_set tid
     end.
   Function trace_conflict_free (tr : trace) : Prop :=
     match tr with
-      | Event t s1 s2 a r :: tl =>
-        Intersection tid (step_writes s1 s2) (trace_writes tl) = Singleton tid t
-        /\ trace_conflict_free tl
+      | Event s1 s2 (t, _, _) :: tl => Intersection tid (step_writes s1 s2) (trace_writes tl)
+                                       = Singleton tid t
+                                       /\ trace_conflict_free tl
       | _ => True
   end.
 
@@ -115,26 +117,34 @@ Section Commutativity.
 End Commutativity.
 
 Section Emulator_Components.
-  Parameter spec : list history.
-  Parameter spec_oracle : history -> bool.
-  Parameter X : history.
-  Parameter Y : history.
-  Parameter base_history : tid -> history.
   Parameter num_threads : nat.
   Parameter num_invocations : nat.
   Parameter num_responses : nat.
-
   Parameter tid_le_num_threads : forall tid, tid < num_threads.
   Parameter inv_types_le_num_invocations :
     forall a n, a = Inv n -> n < num_invocations.
   Parameter resp_types_le_num_resp :
     forall r n, r = Resp n -> n < num_responses.
-  (* XXX *)
-  Hypothesis response_always_exists :
+
+  Parameter spec : list history.
+  Parameter spec_oracle : history -> bool.
+  Parameter X : history.
+  Parameter Y : history.
+  Function get_invocations (h : history) (acc : list (tid * invocation)) :=
+    match h with
+      | [] => acc
+      | (t, i, _) :: tl => get_invocations tl ((t, i) :: acc)
+    end.
+  Definition X_invocations := get_invocations X [].
+  Definition Y_invocations := get_invocations Y [].
+
+  Hypothesis response_always_exists : (* XXX *)
     forall i h t, spec_oracle h = true ->
                  exists r, spec_oracle ((t, i, r) :: h) = true.
   Parameter spec_oracle_correct :
     forall history, List.In history spec <-> spec_oracle history = true.
+
+  Parameter base_history : tid -> history.
   Parameter base_history_well_formed :
     forall t,
       base_history t = X ++ (history_of_thread Y t)
@@ -146,9 +156,11 @@ End Emulator_Components.
 Section Emulator.  
   Definition inc_tid_base_history_pos (bh : tid -> nat) (t: tid) :=
     fun tid => if tid =? t then bh tid + 1 else bh tid.
-  Definition set_tid_mode (mds: mode_state) (t : tid) (md: mode) :=
-    fun tid => if tid =? t then md else mds t.
-  Definition add_to_current_history (ch : current_history_state) (a: action) :=
+  Definition set_all_mode (md: mode) :=
+    fun (t : tid) => md.
+  Definition add_to_tid_current_history (t : tid) (ch : current_history_state) (a : action) :=
+    fun tid => if tid =? t then a :: ch tid else ch tid.    
+  Definition add_to_all_current_histories (ch : current_history_state) (a: action) :=
     fun tid => a :: ch tid. (* note that history goes backward for ease of proof *)
   
   Function combine_histories (ch : current_history_state) (tid : tid)
@@ -159,70 +171,69 @@ Section Emulator.
                                  (* note that we can just stick it on because Y is
                                   * sim-commutative! *)
     end.
-  Definition get_and_set_combined_history (s : state) (base : history) : state :=
-    let '(bh, ch, comm) := get_state_components s in
-    let hcombined := combine_histories ch num_threads base in
-    State bh (fun tid => hcombined) comm.
+  Definition switch_to_emulate (s : state) : state :=
+    let '(bh, ch, mds) := get_state_components s in
+    let hcombined := combine_histories ch num_threads (ch 0) in
+    State bh (fun tid => hcombined) (set_all_mode Emulate).
 
-  Function get_emulate_response_helper (s : state) (a: action) (rt : nat) : state * action :=
+  Function get_emulate_response_helper (s : state) (t: tid) (i : invocation) (rtyp : nat) :
+    state * action :=
     let '(bh, ch, md) := get_state_components s in
-    let t := thread_of_action a in
-    let new_history := ActResp t rt :: a :: (ch t) in
+    let response_action := (t, i, Resp rtyp) in
+    let new_history := response_action :: (ch t) in
     let new_state := State bh (fun tid => new_history) md in
-    if spec_oracle new_history then (new_state, ActResp t rt)
-    else match rt with
-           | 0 => (s, ActResp t 0) (* XXX *)
-           | S rt' => get_emulate_response_helper s a rt'
+    if spec_oracle new_history then (new_state, (t, i, Resp rtyp))
+    else match rtyp with
+           | 0 => (new_state, (t, i, Resp rtyp)) (* XXX *)
+           | S rt' => get_emulate_response_helper s t i rt'
          end.
-  Definition get_emulate_response (s : state) (a : action) : state * action :=
-    get_emulate_response_helper s a num_responses.
-        
-  Definition emulator_act (s : state) (a : action) : (state * action) :=
-    let t := thread_of_action a in
+  Definition get_emulate_response (s : state) (t: tid) (i : invocation) : state * action :=
+    get_emulate_response_helper s t i num_responses.
+
+  Definition get_base_history_response (s : state) (t: tid) (i : invocation) : state * action :=
+    let '(bh, ch, mds) := get_state_components s in
+    let hd := nth_error (base_history t) (bh t) in
+    match hd with
+      | None => let new_state := switch_to_emulate s in
+                get_emulate_response new_state t i
+      | Some bh_action => if action_invocation_eq bh_action i
+                          then let new_state := State (inc_tid_base_history_pos bh t)
+                                                      (add_to_tid_current_history t ch bh_action)
+                                                      mds in                               
+                               (new_state, bh_action)
+                          else let new_state := switch_to_emulate s in
+                               get_emulate_response new_state t i
+    end.
+
+  Definition emulator_act (s : state) (t: tid) (i : invocation) : (state * action) :=
     let '(bh, ch, mds) := get_state_components s in
     match mds t with
-      | Emulate => get_emulate_response s a
-      | Commute => let hd := nth_error (bh t) (base_history t) in
-                   match hd with
-                     | None => switch_to_emulate_and_get_response
-                     | Some bh_action => if 
-    (* get the response and perform emulation if necessary *)
-    let (s_response, r) := if action_eq hd a
-                           then (s', Continue t)
-                           else if action_eq (Continue t) a &&
-                                             is_response hd &&
-                                             (thread_of_action hd =? t)
-                                then (s', hd)
-                                else emulate_mode_and_perform_emulation s' hd t in
-    let '(bh_new, ch_new, comm_new) := get_state_components s_response in
-    let final_bh := if comm_new t
-                    then inc_tid_base_history_pos bh_new t (* conflict-free mode *)
-                    else fun tid => (bh_new tid) + 1 in (* replay mode *) 
-    (State final_bh ch_new comm_new, r).
-  Function emulator_trace_helper (hrun : history) (s0: state) (tr : trace) :=
-    match hrun with
-      | [] => tr
-      | a :: rest => let (s', r) := emulator_act s0 a in
-                     let t := thread_of_action a in
-                     emulator_trace_helper rest s' (Event t s0 s' a r :: tr)
+      | Emulate => get_emulate_response s t i
+      | Commute => get_base_history_response s t i
+      | Replay => let '(State bh' ch' mds', a) := get_base_history_response s t i in
+                  if leb (length X) (bh t)
+                  then (State bh' ch' (set_all_mode Commute), a)
+                  else (State bh' ch' mds', a)
     end.
-  Definition emulator_trace (hrun : history) (s0 : state) : trace :=
-    emulator_trace_helper hrun s0 [].
+  Function emulator_trace_helper (ils : list (tid * invocation)) (s0: state) (tr : trace) :=
+    match ils with
+      | [] => tr
+      | (t, i) :: rest => let (s', a) := emulator_act s0 t i in
+                          emulator_trace_helper rest s' (Event s0 s' a :: tr)
+    end.
+  Definition emulator_trace (ils : list (tid * invocation)) (s0 : state) : trace :=
+    emulator_trace_helper ils s0 [].
 
 End Emulator.
 
 Section Theorems.
   Lemma state_after_X_invocations :
-    forall bh ch comm,
-      Some (State bh ch comm) = trace_end_state (emulator_trace X_invocations start_state) ->
+    forall bh ch mds,
+      Some (State bh ch mds) = trace_end_state (emulator_trace X_invocations start_state) ->
       forall t,
-        nth (bh t) (base_history t) (Emulate t) = Commute t /\
-        ch t = X.
+        mds t = Commute /\ bh t = length X.
   Proof.
   Admitted.
-
-  Lemma state_
-
   
   Lemma trace_conflict_free_cons : forall e tr,
     trace_conflict_free (e :: tr) -> trace_conflict_free tr.
@@ -235,32 +246,22 @@ Section Theorems.
       Some sComm = trace_end_state (emulator_trace X_invocations start_state) ->
       trace_conflict_free (emulator_trace Y_invocations sComm).
   Proof.
-    intros s0 sComm Hs0.
-    pose base_history_well_formed as Hwf.
-    pose spec_oracle_correct as Hspec.
-    remember Y_invocations as yi.
-    unfold Y_invocations in *.
-    induction yi.
-    simpl; auto.
-    
   Admitted.
 
   (* if we have the emulator instantiated with a SIM-comm history,
    * and the emulator acts on some input sequence, then the emulator
    * produces a trace whose corresponding history is correct *)
   Lemma emulator_impl_correct :
-    forall invocations,
-      only_has_invocations invocations ->
-      spec_oracle (history_of_trace (emulator_trace invocations start_state)) = true.
+    forall (ils : list (tid * invocation)),
+      spec_oracle (history_of_trace (emulator_trace ils start_state)) = true.
   Proof.
   Admitted.
 
   Theorem scalable_commutativity_rule :
-    forall sComm invocations,
-      (Some sComm = trace_end_state (emulator_trace X start_state) ->
+    forall sComm ils,
+      (Some sComm = trace_end_state (emulator_trace X_invocations start_state) ->
       trace_conflict_free (emulator_trace Y_invocations sComm))
-      /\ (only_has_invocations invocations ->
-          spec_oracle (history_of_trace (emulator_trace invocations start_state)) = true).
+      /\ spec_oracle (history_of_trace (emulator_trace ils start_state)) = true.
   Proof.
     intros; split; [eapply emulator_impl_conflict_free | eapply emulator_impl_correct]; eauto.
   Qed.
